erasure/theories/Debox.v
@@ -1,0 +1,34 @@
+From MetaCoq Require Import utils.
+From MetaCoq.Erasure Require Import EAst.
+
+Definition get_shift (n : nat) (g : list bool) :=
+  List.count_occ Bool.bool_dec (List.firstn (1+n) g) true.
+
+Fixpoint debox (g : list bool) (t : term) :=
+  match t with
+  | tRel i => tRel (i - get_shift i g)
+  | tEvar ev args => tEvar ev (List.map (debox g) args)
+  | tLambda na M => match na.(binder_erasure_reason) with
+                   | Some ER_type => debox (true :: g) M
+                   | _ => tLambda na (debox (false :: g) M)
+                   end
+  | tApp u v => match v with
+               | tBox ER_type => debox g u
+               | _ => tApp (debox g u) (debox g v)
+               end
+  | tLetIn na b b' => tLetIn na (debox g b) (debox (false :: g) b')
+  | tCase ind c brs =>
+    let brs' := List.map (on_snd (debox g)) brs in
+    tCase ind (debox g c) brs'
+  | tProj p c => tProj p (debox g c)
+  | tFix mfix idx =>
+    let mfix' := List.map (map_def (debox g)) mfix in
+    tFix mfix' idx
+  | tCoFix mfix idx =>
+    let comfix' := List.map (map_def (debox g)) mfix in
+    tCoFix comfix' idx
+  | tBox r => t
+  | tVar _ => t
+  | tConst _ => t
+  | tConstruct _ _ => t
+  end.
