erasure/theories/EInversion.v
@@ -26,13 +26,14 @@ Notation type_tFix_inv := PCUICInversion.inversion_Fix.
 
 Derive Signature for Forall2.
 Lemma eval_box_apps:
-  forall (Σ' : E.global_declarations) (e : E.term) (x x' : list E.term),
+  forall (Σ' : E.global_declarations) (e : E.term) (x x' : list E.term)
+    (r : E.erasure_reason),
     Forall2 (eval Σ') x x' ->
-    eval Σ' e EAst.tBox -> eval Σ' (EAst.mkApps e x) EAst.tBox.
+    eval Σ' e (EAst.tBox r) -> eval Σ' (EAst.mkApps e x) (EAst.tBox r).
 Proof.
   intros Σ' e x H2. revert e H2; induction x using rev_ind; cbn; intros; eauto using eval.
   eapply Forall2_app_inv_l in H as [l1' [l2' [H [H' eq]]]]. subst H2.
   depelim H'.
-  specialize (IHx e _ H H0). simpl.
+  specialize (IHx e _ _ H H0). simpl.
   rewrite mkApps_app. simpl. econstructor; eauto.
 Qed.
